Working on access proofs

Safety.v
@@ -4,88 +4,172 @@ From Coq Require Import Logic.ClassicalFacts.
 
 From Elo Require Export Core0.
 
-Reserved Notation "m / t / tc '==>*' m' / t' / tc'"
+Reserved Notation "m / t '==[' tc ']==>*' m' / t'"
   (at level 40, t at next level, tc at next level,
                 m' at next level, t' at next level).
 
 Definition trace := list effect.
 
-Inductive has_access (m : mem) : tm -> addr -> Prop :=
-  | has_access_trans : forall t ad ad',
+Inductive access (m : mem) : tm -> addr -> Prop :=
+  | access_trans : forall t ad ad',
+    access m t ad ->
     get_tm m ad = TM_Loc ad' ->
-    has_access m t ad ->
-    has_access m t ad'
+    access m t ad'
 
-  | has_access_loc : forall ad,
-    has_access m (TM_Loc ad) ad
+  | access_loc : forall ad,
+    access m (TM_Loc ad) ad
 
-  | has_access_new : forall t ad,
-    has_access m t ad ->
-    has_access m (TM_New t) ad
+  | access_new : forall t ad,
+    access m t ad ->
+    access m (TM_New t) ad
 
-  | has_access_load : forall t ad,
-    has_access m t ad ->
-    has_access m (TM_Load t) ad
+  | access_load : forall t ad,
+    access m t ad ->
+    access m (TM_Load t) ad
 
-  | has_access_asg1 : forall l r ad,
-    has_access m l ad ->
-    has_access m (TM_Asg l r) ad
+  | access_asg1 : forall l r ad,
+    access m l ad ->
+    access m (TM_Asg l r) ad
 
-  | has_access_asg2 : forall l r ad,
-    has_access m r ad ->
-    has_access m (TM_Asg l r) ad
+  | access_asg2 : forall l r ad,
+    access m r ad ->
+    access m (TM_Asg l r) ad
   .
 
-Theorem aux1 : forall m t t' ad v,
-  t' --[EF_Alloc ad v]--> t ->
-  has_access m t ad.
+Inductive multistep : mem -> tm -> trace -> mem -> tm -> Prop :=
+  | multistep_refl : forall m t tc,
+    m / t ==[tc]==>* m / t
+
+  | multistep_step : forall m m' m'' t t' t'' tc eff,
+    m  / t  ==[tc       ]==>* m'  / t'  ->
+    m' / t' ==[eff      ]==>  m'' / t'' ->
+    m  / t  ==[eff :: tc]==>* m'' / t''
+
+  where "m / t '==[' tc ']==>*' m' / t'" := (multistep m t tc m' t').
+
+Lemma alloc_grants_access_1 : forall m m' t t' ad v,
+  ~ (access m t ad) ->
+  t --[EF_Alloc ad v]--> t' ->
+  access m' t' ad.
 Proof.
-  intros ? ? ?. generalize dependent t.
-  induction t'; intros * Hstep;
-  inversion Hstep; eauto using has_access.
+  intros ? ? ?. induction t; intros * Hacc Hstep;
+  inversion Hstep; eauto using access.
+  - eapply access_load; eauto using access.
+  - eapply access_asg1; eauto using access.
+  - eapply access_asg2; eauto using access.
 Qed.
 
-Inductive multistep : mem -> tm -> trace -> mem -> tm -> trace -> Prop :=
-  | multistep_first : forall main ad,
-    ~ (has_access nil main ad) ->
-    nil / TM_Nil / nil ==>* nil / main / (EF_None :: nil)
+Lemma alloc_grants_access_2 : forall m m' t t' ad v,
+  ~ (access m t ad) ->
+  m / t ==[EF_Alloc ad v]==> m' / t' ->
+  access m' t' ad.
+Proof.
+  intros * Hacc Hmstep. destruct t';
+  inversion Hmstep; subst; eauto using alloc_grants_access_1.
+Qed.
 
-  | multistep_step : forall m m' m'' t t' t'' tc tc' ceff,
-    m  / t / tc ==>* m' / t' / tc' ->
-    m' / t' ==[ceff]==> m'' / t'' ->
-    m  / t / tc ==>* m'' / t'' / (ceff :: tc')
-
-  where "m / t / tc '==>*' m' / t' / tc'" := (multistep m t tc m' t' tc').
-
-
-
-
-
-
-
+Lemma alloc_grants_access_3 : forall m m' tc t t' ad v,
+  ~ (access m t ad) ->
+  m / t ==[EF_Alloc ad v :: tc]==>* m' / t' ->
+  access m' t' ad.
+Proof.
+  intros * Hacc Hmultistep. inversion Hmultistep; subst.
+  -
+  - inversion Hmultistep; subst.
+    + inversion Hmultistep.
+  inversion Hmultistep; subst; eauto using alloc_grants_access_2.
+Qed.
 
 
 
-Lemma ceff_eq_dec : forall (x y : ceffect),
-  x = y \/ x <> y.
+Lemma eff_eq_dec : forall (x y : effect),
+  {x = y} + {x <> y}.
+Proof.
 Admitted.
 
-Theorem todo : forall m_ m ths_ ths tc_ tc tid ad v,
-  m_ / ths_ / tc_ ==>* m / ths / (CEF_Load tid ad v :: tc) ->
-  In (CEF_Alloc tid ad v) tc.
+Definition NotIn {A} (a : A) l := ~ (In a l).
+
+Lemma duplicate_alloc' : forall {m m' t t'} tc {ad v},
+  m / t / tc ==>* m' / t' / (EF_Alloc ad v :: tc) ->
+  NotIn (EF_Alloc ad v) tc.
+Proof.
+  unfold NotIn. intros * Hmstep. induction Hmstep; eauto using in_nil.
+Qed.
+
+Lemma duplicate_alloc : forall m m' t t' tc tc' ad v,
+  m / t / tc ==>* m' / t' / (EF_Alloc ad v :: tc') ->
+  ~ (In (EF_Alloc ad v) tc').
+Proof.
+  intros * Hmstep. destruct tc' as [| x xs].
+  - eauto using in_nil.
+  - destruct (eff_eq_dec (EF_Alloc ad v) x).
+    + subst. destruct (list_eq_dec eff_eq_dec xs tc).
+      * subst. exfalso. eapply (duplicate_alloc'). eapply Hmstep.
+      * 
+Qed.
+
+Lemma aux1 : forall {A} l1 l2 (a : A), 
+  (~ (In a (l1 ++ l2))) = ~ (In a l1) /\ ~ (In a l2).
+Proof.
+Admitted.
+
+Lemma duplicate_alloc : forall m m' t t' tc tc' ad v,
+  m / t / tc ==>* m' / t' / (EF_Alloc ad v :: tc') ->
+  ~ (In (EF_Alloc ad v) tc').
 Proof.
   intros * Hmstep.
-  inversion Hmstep. subst.
+  assert (exists x, tc' = x ++ tc) as [x Htc]. { shelve. } subst.
+  erewrite aux1. split.
+  - destruct x as [| x xs].
+    + eauto using in_nil.
+    + destruct (eq_dec_eff (EF_Alloc ad v) x).
+      * shelve.
+      * eapply not_in_cons. split; auto.
+        inversion Hmstep; subst.
+        inversion H6; subst.
+        ** erewrite app_nil_r in H8. subst. eauto using in_nil.
+        ** induction xs.
+          *** shelve.
+          ***
+  - eauto using duplicate_alloc'.
+Qed.
 
 
 
 
-induction tc as [| ceff tc' IH].
-  - inversion Hmstep; subst. inversion H6.
-  - destruct (ceff_eq_dec ceff (CEF_Alloc tid ad v)); subst.
+
+Lemma aux1 : forall m m' t t' tc tc' tc'' eff,
+  m' / t' / tc' ==>* m / t / (eff :: tc) ->
+  m' / t' / tc' ==>* m / t / ((eff :: tc'') ++ tc').
+Proof.
+Admitted.
+
+Lemma in_dec_eff : forall (eff : effect) (l : list effect),
+  {In eff l} + {~ In eff l}.
+Proof.
+  intros *. eauto using in_dec, eq_dec_eff.
+Qed.
+
+Theorem todo : forall m m' t t' tc tc' ad v,
+  m' / t' / tc' ==>* m / t / (EF_Load ad v :: tc) ->
+  In (EF_Alloc ad v) tc.
+Proof.
+  intros * Hmstep.
+  assert (In1 : {In (EF_Alloc ad v) tc} + {~ In (EF_Alloc ad v) tc}).
+  eauto using in_dec_eff. destruct In1 as [In1 | NIn1].
+  - auto.
+  - assert (In2 : {In (EF_Alloc ad v) tc'} + {~ In (EF_Alloc ad v) tc'}).
+    eauto using in_dec_eff. destruct In2 as [In2 | NIn2].
+    + auto.
+    +
+
+
+  induction tc_ as [| ceff tc' IH].
+  - inversion Hmstep; subst.
+  - destruct (ceff_eq_dec ceff (EF_Alloc ad v)); subst.
     + eapply in_eq.
     + eapply in_cons. clear H.
-      inversion Hmstep. subst.
+      inversion Hmstep; subst.
       inversion H6; subst.
       * shelve.
       *
